tentative equations between state-trace and state and trace

trace_monad.v
@@ -13,6 +13,7 @@ Unset Printing Implicit Defensive.
 (*
 Contents:
 - Module MonadTrace.
+- Module MonadTraceRun.
 - Module MonadStateTrace.
 - Module MonadStateTraceRun.
 - wip
@@ -40,6 +41,46 @@ Export MonadTrace.Exports.
 
 Definition marks T {M : traceMonad T} (l : seq T) : M (seq unit) :=
   sequence (map Mark l).
+
+Module MonadTraceRun.
+Record mixin_of T (M : traceMonad T) : Type := Mixin {
+  run : forall A, M A -> seq T -> A * seq T ;
+  _ : forall A (a : A) s, run (Ret a) s = (a, s) ;
+  _ : forall A B (m : M A) (f : A -> M B) s,
+    run (do a <- m ; f a) s =
+    let (a', s') := run m s in run (f a') s' ;
+  _ : forall t l, run (Mark t) l = (tt, l ++ t :: nil) (* TODO: rcons *)
+}.
+Record class_of T (m : Type -> Type) : Type := Class {
+  base : MonadTrace.class_of T m ;
+  mixin : mixin_of (MonadTrace.Pack base)
+}.
+Structure t T : Type := Pack { m : Type -> Type ;
+  class : class_of T m }.
+Definition op_run T (M : t T) : forall A, m M A -> seq T -> A * seq T :=
+  let: Pack _ (Class _ (@Mixin _ _ x _ _ _)) := M
+  return forall A, m M A -> seq T -> A * seq T in x.
+Arguments op_run {T M A} : simpl never.
+Definition baseType T (M : t T) := MonadTrace.Pack (base (class M)).
+Module Exports.
+Notation Runt := op_run.
+Notation traceRunMonad := t.
+Coercion baseType T (M : traceRunMonad T) : traceMonad T := baseType M.
+Canonical baseType.
+End Exports.
+End MonadTraceRun.
+Export MonadTraceRun.Exports.
+
+Section tracerun_lemmas.
+Variables (S : Type) (M : traceRunMonad S).
+Lemma runtret : forall A (a : A) s, Runt (Ret a : M _) s = (a, s).
+Proof. by case: M => m [? []]. Qed.
+Lemma runtbind : forall A B (ma : M A) (f : A -> M B) s,
+  Runt (do a <- ma ; f a) s = let: (a'', s'') := Runt ma s in Runt (f a'') s''.
+Proof. by case: M => m [? []]. Qed.
+Lemma runtmark : forall s t, Runt (Mark t : M _) s = (tt, s ++ t :: nil). (* TODO: rcons *)
+Proof. by case: M => m [? []]. Qed.
+End tracerun_lemmas.
 
 Module MonadStateTrace.
 Record mixin_of S T (M : monad) : Type := Mixin {
@@ -105,7 +146,7 @@ Record mixin_of S T (M : stateTraceMonad S T) : Type := Mixin {
     let: (a', s') := run m s in run (f a') s' ;
   _ : forall s l, run stGet (s, l) = (s, (s, l)) ;
   _ : forall s l s', run (stPut s') (s, l) = (tt, (s', l)) ;
-  _ : forall t s l, run (stMark t) (s, l) = (tt, (s, l ++ [:: t]))
+  _ : forall t s l, run (stMark t) (s, l) = (tt, (s, l ++ t :: nil)) (* TODO: rcons *)
 }.
 Record class_of S T (m : Type -> Type) : Type := Class {
   base : MonadStateTrace.class_of S T m ;
@@ -129,19 +170,70 @@ Export MonadStateTraceRun.Exports.
 
 Section statetracerun_lemmas.
 Variables (S T : Type) (M : stateTraceRunMonad S T).
-Lemma runret : forall A (a : A) s, Run (Ret a : M _) s = (a, s).
+Lemma runstret : forall A (a : A) s, Run (Ret a : M _) s = (a, s).
 Proof. by case: M => m [? []]. Qed.
-Lemma runbind : forall A B (ma : M A) (f : A -> M B) s,
+Lemma runstbind : forall A B (ma : M A) (f : A -> M B) s,
   Run (do a <- ma ; f a) s =
   let: (a'', s'') := Run ma s in Run (f a'') s''.
 Proof. by case: M => m [? []]. Qed.
-Lemma runget : forall s l, Run (stGet : M _) (s, l) = (s, (s, l)).
+Lemma runstget : forall s l, Run (stGet : M _) (s, l) = (s, (s, l)).
 Proof. by case: M => m [? []]. Qed.
-Lemma runput : forall s l s', Run (stPut s' : M _) (s, l) = (tt, (s', l)).
+Lemma runstput : forall s l s', Run (stPut s' : M _) (s, l) = (tt, (s', l)).
 Proof. by case: M => m [? []]. Qed.
-Lemma runmark : forall t s l, Run (stMark t : M _) (s, l) = (tt, (s, l ++ [:: t])).
+Lemma runstmark : forall t s l, Run (stMark t : M _) (s, l) = (tt, (s, l ++ t :: nil)). (* TODO: rcons *)
 Proof. by case: M => m [? []]. Qed.
 End statetracerun_lemmas.
+
+Definition mkStateTraceMonad {S T} : stateTraceMonad S T.
+refine (
+let m := (@Monad.Class (fun A => S * list T -> A * (S * list T))
+  (fun A a => fun s => (a, s)) (* ret *)
+  (fun A B m f => fun s => let (a, s') := m s in f a s') (* bind *) _ _ _) in
+let stm := (@MonadStateTrace.Class S T _ m
+  (@MonadStateTrace.Mixin _ _ (Monad.Pack m)
+  (fun s => (s.1, s))  (* get *)
+  (fun s' s => (tt, (s', s.2)))
+  (fun (t : T) s => (tt, (s.1, s.2 ++ t :: nil))))) in
+@MonadStateTrace.Pack S T (fun A => S * list T -> A * (S * list T)) stm).
+by [].
+move=> A f; apply functional_extensionality => ?; by case: f.
+move=> A B C a b c; apply functional_extensionality => ?; by case: a.
+Defined.
+
+Definition mkStateTraceRunMonad {S T} :
+  stateTraceRunMonad S T.
+exact: (let stm := mkStateTraceMonad in
+@MonadStateTraceRun.Pack S T (fun A => S * list T -> A * (S * list T))
+  (@MonadStateTraceRun.Class S T (fun A => S * list T -> A * (S * list T))
+    (MonadStateTrace.class stm)
+    (@MonadStateTraceRun.Mixin _ _ stm
+      (fun A m (s : S * list T) => m s) (* run *) _ _ _ _ _))).
+Defined.
+
+Definition assoc {A B C : Type} (x : (A * B) * C) : A * (B * C) :=
+(fst (fst x), (snd (fst x), snd x)).
+
+Definition assoc_inv {A B C : Type} (x : A * (B * C)) : (A * B) * C :=
+((fst x, fst (snd x)), snd (snd x)).
+
+Section tmp.
+Variables (S T : Type).
+Let MN := @mkStateTraceRunMonad S T.
+
+Lemma stGet_Get (M : stateRunMonad S) s :
+  Run (stGet : MN _) s = assoc (Run0 (Get : M _) s.1, s.2).
+Proof. rewrite state_monad.runget; by case: s. Qed.
+
+Lemma stPut_Put (M : stateRunMonad S) s s' :
+  Run (stPut s' : MN _) s = assoc (Run0 (Put s' : M _) s.1, s.2).
+Proof. by rewrite state_monad.runput. Qed.
+
+Lemma stMark_Mark (M : traceRunMonad T) s t :
+  Run (stMark t : MN _) s =
+    let x := Runt (Mark t : M _) s.2 in (x.1, (s.1, x.2)).
+Proof. by rewrite runtmark. Qed.
+
+End tmp.
 
 (* WIP *)
 
